ebpf/Size.v
@@ -1,0 +1,22 @@
+(* *********************************************************************)
+(*           Check range                                               *)
+(*       Frédéric Besson (frederic.besson@inria.fr), Inria Rennes      *)
+(* *********************************************************************)
+
+Require Import Coqlib Errors Maps.
+Require Import AST Zbits Integers Floats Values Memory Globalenvs.
+
+Module Ptrofs.
+
+  Definition is_16_signed (p:ptrofs) :=
+    let i := Ptrofs.signed p in
+    Z.leb (-(2^15)) i && Z.leb i (2^15 - 1).
+
+  Definition is_int (n:ptrofs) :=
+    if negb Archi.ptr64 then true
+    else
+      let i := Ptrofs.signed n in
+      Z.leb Int.min_signed i && Z.leb i Int.max_signed.
+
+
+End Ptrofs.
